Renamed the three Sponge theories:
  TopLevel => Sponge
  Block    => BlockSponge
  Absorb   => AbsorbSponge

Added injectivity lemma for pad2blocks to Common.

Fixed a glitch in the game structure of Sponge (was TopLevel).  Also
got rid of smt (without ml=0) calls.

sha3/proof/Sponge.ec
@@ -2,7 +2,7 @@
 
 require import Fun Pair Int IntDiv Real List Option FSet NewFMap DBool.
 require import Common StdOrder. import IntOrder.
-require (*--*) IRO Block.
+require (*--*) IRO BlockSponge.
 
 (*------------------------- Indifferentiability ------------------------*)
 
@@ -53,7 +53,7 @@ module Sponge (P : DPRIMITIVE) : FUNCTIONALITY, CONSTRUCTION(P) = {
 
 (*------------- Simulator and Distinguisher Constructions --------------*)
 
-module LowerFun (F : DFUNCTIONALITY) : Block.DFUNCTIONALITY = {
+module LowerFun (F : DFUNCTIONALITY) : BlockSponge.DFUNCTIONALITY = {
   proc f(xs : block list, n : int) = {
     var cs, ds : bool list;
     var obs : bool list option;
@@ -68,7 +68,7 @@ module LowerFun (F : DFUNCTIONALITY) : Block.DFUNCTIONALITY = {
   }
 }.
 
-module RaiseFun (F : Block.DFUNCTIONALITY) : DFUNCTIONALITY = {
+module RaiseFun (F : BlockSponge.DFUNCTIONALITY) : DFUNCTIONALITY = {
   proc f(bs : bool list, n : int) = {
     var xs;
 
@@ -77,16 +77,18 @@ module RaiseFun (F : Block.DFUNCTIONALITY) : DFUNCTIONALITY = {
   }
 }.
 
-module LowerDist (D : DISTINGUISHER, F : Block.DFUNCTIONALITY) = D(RaiseFun(F)).
+module LowerDist (D : DISTINGUISHER, F : BlockSponge.DFUNCTIONALITY) =
+  D(RaiseFun(F)).
 
-module RaiseSim (S : Block.SIMULATOR, F : DFUNCTIONALITY) = S(LowerFun(F)).
+module RaiseSim (S : BlockSponge.SIMULATOR, F : DFUNCTIONALITY) =
+  S(LowerFun(F)).
 
 (*------------------------------- Proof --------------------------------*)
 
 section.
 
-declare module BlockSim  : Block.SIMULATOR{IRO, Block.BIRO.IRO}.
-declare module Dist : DISTINGUISHER{Perm, BlockSim, IRO, Block.BIRO.IRO}.
+declare module BlockSim  : BlockSponge.SIMULATOR{IRO, BlockSponge.BIRO.IRO}.
+declare module Dist : DISTINGUISHER{Perm, BlockSim, IRO, BlockSponge.BIRO.IRO}.
 
 module type BLOCK_IRO_BITS = {
   proc init() : unit
@@ -95,10 +97,10 @@ module type BLOCK_IRO_BITS = {
 }.
 
 module type BLOCK_IRO_BITS_DIST(BIROB : BLOCK_IRO_BITS) = {
-  proc distinguish(): bool 
+  proc distinguish(): bool {BIROB.g BIROB.f}
 }.
 
-local module BlockIROBitsEager : BLOCK_IRO_BITS, Block.BIRO.IRO = {
+local module BlockIROBitsEager : BLOCK_IRO_BITS, BlockSponge.BIRO.IRO = {
   var mp : (block list * int, bool) fmap
 
   proc init() : unit = {
@@ -140,7 +142,7 @@ local module BlockIROBitsEager : BLOCK_IRO_BITS, Block.BIRO.IRO = {
   }
 }.
 
-local module BlockIROBitsLazy : BLOCK_IRO_BITS, Block.BIRO.IRO = {
+local module BlockIROBitsLazy : BLOCK_IRO_BITS, BlockSponge.BIRO.IRO = {
   var mp : (block list * int, bool) fmap
 
   proc init() : unit = {
@@ -177,6 +179,14 @@ local module BlockIROBitsLazy : BLOCK_IRO_BITS, Block.BIRO.IRO = {
   }
 }.
 
+local lemma BlockIROBitsEager (D <: BLOCK_IRO_BITS_DIST) :
+  equiv[D(BlockIROBitsEager).distinguish ~ D(BlockIROBitsLazy).distinguish : 
+        ={glob D} /\ BlockIROBitsEager.mp{1} = BlockIROBitsLazy.mp{2} ==>
+        ={glob D}].
+proof.
+admit. (* use RndO.ec result *)
+qed.
+
 local module RaiseBIROBLazy (F : BLOCK_IRO_BITS) : FUNCTIONALITY = {
   proc init() = {
     F.init();
@@ -200,6 +210,60 @@ pred LazyInvar
   (forall (bs : bool list, n : int),
    mem (dom mp1) (bs, n) =>
    oget mp1.[(bs, n)] = oget mp2.[(pad2blocks bs, n)]).
+
+local lemma lazy_invar_upd_mem_dom_iff
+      (mp1 : (bool list * int, bool) fmap,
+       mp2 : (block list * int, bool) fmap,
+       bs cs : bool list, n m : int, b : bool) :
+  LazyInvar mp1 mp2 =>
+  mem (dom mp1.[(bs, n) <- b]) (cs, m) <=>
+  mem (dom mp2.[(pad2blocks bs, n) <- b]) (pad2blocks cs, m).
+proof.
+move=> LI; split=> [mem_upd_mp1 | mem_upd_mp2].
+rewrite domP in_fsetU1; rewrite domP in_fsetU1 in mem_upd_mp1.
+case: ((cs, m) = (bs, n))=> [cs_m_eq_bs_n | cs_m_neq_bs_n].
+right; by elim cs_m_eq_bs_n=> ->->.
+left; smt ml=0.
+rewrite domP in_fsetU1; rewrite domP in_fsetU1 in mem_upd_mp2.
+case: ((cs, m) = (bs, n))=> [// | cs_m_neq_bs_n].
+elim mem_upd_mp2=> [/# | [p2b_cs_p2b_bs eq_mn]].
+have /# : cs = bs by apply pad2blocks_inj.
+qed.
+
+local lemma lazy_invar_upd2_vb
+      (mp1 : (bool list * int, bool) fmap,
+       mp2 : (block list * int, bool) fmap,
+       bs : bool list, xs : block list, n m : int, b : bool) :
+  LazyInvar mp1 mp2 =>
+  mem (dom mp2.[(pad2blocks bs, n) <- b]) (xs, m) =>
+  valid_block xs.
+proof.
+move=> LI mem_upd_mp2.
+rewrite domP in_fsetU1 in mem_upd_mp2.
+elim mem_upd_mp2=> [/# | [-> _]].
+apply/valid_pad2blocks.
+qed.
+
+local lemma lazy_invar_upd_lu_eq
+      (mp1 : (bool list * int, bool) fmap,
+       mp2 : (block list * int, bool) fmap,
+       bs cs : bool list, n m : int, b : bool) :
+  LazyInvar mp1 mp2 =>
+  mem (dom mp1.[(bs, n) <- b]) (cs, m) =>
+  oget mp1.[(bs, n) <- b].[(cs, m)] =
+  oget mp2.[(pad2blocks bs, n) <- b].[(pad2blocks cs, m)].
+proof.
+move=> LI mem_upd_mp1.
+case: ((cs, m) = (bs, n))=> [[->->] | cs_m_neq_bs_n].
+smt ml=0 w=(getP_eq).
+rewrite domP in_fsetU1 in mem_upd_mp1.
+elim mem_upd_mp1=> [mem_mp1 | [->->]].
+case: ((pad2blocks bs, n) = (pad2blocks cs, m))=>
+  [[p2b_bs_p2b_cs eq_mn] | p2b_bs_n_neq_p2b_cs_m].
+smt ml=0 w=(pad2blocks_inj).
+smt ml=0 w=(getP).
+smt ml=0 w=(getP).
+qed.
 
 local lemma LowerFun_IRO_BlockIROBitsLazy_f :
   equiv[LowerFun(IRO).f ~ BlockIROBitsLazy.f :
@@ -226,8 +290,13 @@ while
 sp; auto.
 if.
 progress; smt ml=0.
-rnd; auto; progress; smt. (* will get rid of smt's *)
-auto; progress; smt.
+rnd; auto; progress;
+  [smt ml=0 w=(getP_eq) |
+   smt ml=0 w=(lazy_invar_upd_mem_dom_iff) |
+   smt ml=0 w=(lazy_invar_upd_mem_dom_iff) |
+   smt ml=0 w=(lazy_invar_upd2_vb) |
+   smt ml=0 w=(lazy_invar_upd_lu_eq)].
+auto; progress; smt ml=0.
 auto.
 rcondf{1} 3; first auto. rcondf{2} 4; first auto.
 auto; progress; by rewrite bits2blocks_nil.
@@ -251,18 +320,15 @@ while
    LazyInvar IRO.mp{1} BlockIROBitsLazy.mp{2}).
 wp; sp.
 if.
-progress; smt.  (* will get rid of smt's *)
-rnd; skip; progress; smt.
-auto; progress; smt.
+progress; smt ml=0.
+rnd; skip; progress;
+  [smt ml=0 w=(getP_eq) |
+   smt ml=0 w=(lazy_invar_upd_mem_dom_iff) |
+   smt ml=0 w=(lazy_invar_upd_mem_dom_iff) |
+   smt ml=0 w=(lazy_invar_upd2_vb) |
+   smt ml=0 w=(lazy_invar_upd_lu_eq)].
+auto; progress; smt ml=0.
 auto.
-qed.
-
-local lemma BlockIROBitsEager (D <: BLOCK_IRO_BITS_DIST) :
-  equiv[D(BlockIROBitsEager).distinguish ~ D(BlockIROBitsLazy).distinguish : 
-        ={glob D} /\ BlockIROBitsEager.mp{1} = BlockIROBitsLazy.mp{2} ==>
-        ={glob D}].
-proof.
-admit. (* use RndO.ec result *)
 qed.
 
 pred EagerInvar
@@ -278,48 +344,119 @@ pred EagerInvar
    mem (dom mp2) (xs, j) =>
    0 <= j /\ mem (dom mp1) (xs, j %/ r)).
 
-local lemma BlockIROBitsEager_BlockIRO_f :
-  equiv[BlockIROBitsEager.f ~ Block.BIRO.IRO.f :
-        xs{1} = x{2} /\ ={n} /\
-        EagerInvar Block.BIRO.IRO.mp{2} BlockIROBitsEager.mp{1} ==>
-        ={res} /\ EagerInvar Block.BIRO.IRO.mp{2} BlockIROBitsEager.mp{1}].
+local lemma BlockIROBitsEager_f_BlockIRO_g :
+  equiv[BlockIROBitsEager.f ~ BlockIROBitsEager.g :
+        ={xs, BlockIROBitsEager.mp} /\ n{1} * r = n{2} ==>
+        res{1} = bits2blocks res{2} /\ ={BlockIROBitsEager.mp}].
 proof.
-proc=> /=.
-inline BlockIROBitsEager.g.
-seq 5 2 :
-  (={i} /\ xs0{1} = x{2} /\ bs0{1} = [] /\ bs{2} = [] /\ n0{1} = n{2} * r /\
-   n0{1} = m{1} /\
-   EagerInvar Block.BIRO.IRO.mp{2} BlockIROBitsEager.mp{1}).
-auto; progress.
-rewrite -addzA divzMDl 1:gtr_eqF 1:gt0_r //.
-have -> // : (r - 1) %/ r = 0 by smt. (* TODO *)
-if=> //.
-rcondf{1} 2; auto; first while (true); auto.
-conseq
-  (_ :
-   ={i} /\ n0{1} = n{2} * r /\ xs0{1} = x{2} /\ bs0{1} = [] /\ bs{2} = [] /\
-   EagerInvar Block.BIRO.IRO.mp{2} BlockIROBitsEager.mp{1} ==>
-  bits2blocks bs0{1} = bs{2} /\
-  EagerInvar Block.BIRO.IRO.mp{2} BlockIROBitsEager.mp{1})=> //.
-admit.
-auto; progress; by rewrite bits2blocks_nil.
+proc=> /=; inline *.
+seq 5 3 :
+  (={i, BlockIROBitsEager.mp} /\ xs0{1} = xs{2} /\
+   bs0{1} = bs{2} /\ n0{1} = n{2} /\ m{1} = n0{1} /\ m{2} = n{2}).
+auto; progress;
+  first 2 rewrite -addzA divzMDl 1:gtr_eqF 1:gt0_r // divz_small //;
+          smt ml=0 w=(gt0_n).
+if=> //; wp.
+while
+  (={i, BlockIROBitsEager.mp} /\ xs0{1} = xs{2} /\
+   bs0{1} = bs{2} /\ n0{1} = n{2} /\ m{1} = n0{1} /\
+   m{2} = n{2}).
+sp; wp; if=> //; rnd; auto.
+while
+  (={i, BlockIROBitsEager.mp} /\ xs0{1} = xs{2} /\
+   bs0{1} = bs{2} /\ n0{1} = n{2} /\ m{1} = n0{1} /\
+   m{2} = n{2})=> //.
+sp; wp; if=> //; rnd; auto.
+auto.
 qed.
 
-local lemma RaiseFun_BlockIROBitsEager_BlockIRO_f :
-  equiv[RaiseFun(BlockIROBitsEager).f ~ RaiseFun(Block.BIRO.IRO).f :
-        ={bs, n} /\
-        EagerInvar Block.BIRO.IRO.mp{2} BlockIROBitsEager.mp{1} ==>
-        ={res} /\
-        EagerInvar Block.BIRO.IRO.mp{2} BlockIROBitsEager.mp{1}].
+local lemma BlockIROBitsEager_g_Block_IRO_f
+            (n' : int) (x' : block list) :
+  equiv[BlockIROBitsEager.g ~ BlockSponge.BIRO.IRO.f :
+        n' = n{1} /\ xs{1} = x{2} /\ x' = x{2} /\
+        n{2} = (n{1} + r - 1) %/ r /\
+        EagerInvar BlockSponge.BIRO.IRO.mp{2} BlockIROBitsEager.mp{1} ==>
+        EagerInvar BlockSponge.BIRO.IRO.mp{2} BlockIROBitsEager.mp{1} /\
+        (valid_block x' =>
+         res{1} = take n' (blocks2bits res{2}) /\
+         size res{2} = (n' + r - 1) %/ r) /\
+        (! valid_block x' => res{1} = [] /\ res{2} = [])].
 proof.
-proc=> /=; by call BlockIROBitsEager_BlockIRO_f.
+proc=> /=.
+seq 3 2 :
+  (n' = n{1} /\ xs{1} = x{2} /\ x' = x{2} /\
+   n{2} = (n{1} + r - 1) %/ r /\ n{2} * r = m{1} /\
+   i{1} = 0 /\ i{2} = 0 /\ bs{1} = [] /\ bs{2} = [] /\
+  EagerInvar BlockSponge.BIRO.IRO.mp{2} BlockIROBitsEager.mp{1}).
+auto; progress.
+if=> //.
+conseq
+  (_ :
+   xs{1} = x{2} /\ n' = n{1} /\ n{2} = (n{1} + r - 1) %/ r /\
+   n{2} * r = m{1} /\ n{1} <= m{1} /\
+   i{1} = 0 /\ i{2} = 0 /\ bs{1} = [] /\ bs{2} = [] /\
+   EagerInvar BlockSponge.BIRO.IRO.mp{2} BlockIROBitsEager.mp{1} ==>
+   bs{1} = take n' (blocks2bits bs{2}) /\
+   size bs{2} = (n' + r - 1) %/ r /\
+   EagerInvar BlockSponge.BIRO.IRO.mp{2} BlockIROBitsEager.mp{1})=> //.
+progress; apply/needed_blocks_suff.
+admit.   
+qed.
+
+local lemma BlockIROBitsEager_BlockIRO_f :
+  equiv[BlockIROBitsEager.f ~ BlockSponge.BIRO.IRO.f :
+        xs{1} = x{2} /\ ={n} /\
+        EagerInvar BlockSponge.BIRO.IRO.mp{2} BlockIROBitsEager.mp{1} ==>
+        ={res} /\ EagerInvar BlockSponge.BIRO.IRO.mp{2} BlockIROBitsEager.mp{1}].
+proof.
+transitivity
+  BlockIROBitsEager.g
+  (={xs, BlockIROBitsEager.mp} /\ n{2} = n{1} * r /\
+   EagerInvar BlockSponge.BIRO.IRO.mp{2} BlockIROBitsEager.mp{1} ==>
+   res{1} = bits2blocks res{2} /\ ={BlockIROBitsEager.mp})
+  (xs{1} = x{2} /\ n{1} = n{2} * r /\
+   EagerInvar BlockSponge.BIRO.IRO.mp{2} BlockIROBitsEager.mp{1} ==>
+   res{1} = (blocks2bits res{2}) /\
+   EagerInvar BlockSponge.BIRO.IRO.mp{2} BlockIROBitsEager.mp{1}).
+progress.
+exists BlockSponge.BIRO.IRO.mp{2}, BlockIROBitsEager.mp{1}, (xs{1}, n{1} * r).
+  progress; by rewrite H0.
+progress; apply blocks2bitsK.
+conseq BlockIROBitsEager_f_BlockIRO_g.
+progress; by rewrite H0.
+exists* n{1}; elim*=> n1. exists* xs{1}; elim*=> xs'.
+conseq (BlockIROBitsEager_g_Block_IRO_f n1 xs')=> //.
+progress; rewrite H0; by rewrite needed_blocks_prod_r.
+progress.
+case (valid_block xs{1})=> [vb_xs1 | not_vb_xs1].
+have [-> size_result_R] := H3 vb_xs1.
+have -> : n{1} = size(blocks2bits result_R)
+  by rewrite size_blocks2bits size_result_R H0
+             needed_blocks_prod_r mulzC.
+by rewrite take_size.
+by have [->->] := H4 not_vb_xs1.
+qed.
+
+local lemma RaiseBIROBLazy_BlockIROBitsEager_RaiseFun_Block_IRO_f :
+  equiv[RaiseBIROBLazy(BlockIROBitsEager).f ~ RaiseFun(BlockSponge.BIRO.IRO).f :
+  ={bs, n} /\ ={glob BlockSim} /\
+  EagerInvar BlockSponge.BIRO.IRO.mp{2} BlockIROBitsEager.mp{1} ==>
+  ={res} /\ ={glob BlockSim} /\
+  EagerInvar BlockSponge.BIRO.IRO.mp{2} BlockIROBitsEager.mp{1}].
+proof.
+proc=> /=.
+exists* n{1}; elim*=> n'.
+exists* (pad2blocks bs{2}); elim*=> xs2.
+call (BlockIROBitsEager_g_Block_IRO_f n' xs2).
+auto; progress.
+by have [-> _] := H2 _; first apply/valid_pad2blocks.
 qed.
 
 local lemma Sponge_Raise_Block_Sponge_f :
-  equiv[Sponge(Perm).f ~ RaiseFun(Block.Sponge(Perm)).f :
+  equiv[Sponge(Perm).f ~ RaiseFun(BlockSponge.Sponge(Perm)).f :
         ={bs, n, glob Perm} ==> ={res, glob Perm}].
 proof.
-proc; inline Block.Sponge(Perm).f.
+proc; inline BlockSponge.Sponge(Perm).f.
 conseq (_ : ={bs, n, glob Perm} ==> _)=> //.
 swap{2} [3..5] -2.
 seq 4 4 :
@@ -344,8 +481,8 @@ qed.
 
 local lemma RealIndif &m :
   Pr[RealIndif(Sponge, Perm, Dist).main() @ &m: res] =
-  Pr[Block.RealIndif
-     (Block.Sponge, Perm, LowerDist(Dist)).main() @ &m : res].
+  Pr[BlockSponge.RealIndif
+     (BlockSponge.Sponge, Perm, LowerDist(Dist)).main() @ &m : res].
 proof.
 byequiv=> //; proc.
 seq 2 2 : (={glob Dist, glob Perm}); first sim.
@@ -371,7 +508,7 @@ call
   IRO.mp{1} = map0 /\ BlockIROBitsLazy.mp{2} = map0 ==>
   ={res}).
 proc (={glob BlockSim} /\ LazyInvar IRO.mp{1} BlockIROBitsLazy.mp{2}).
-smt.  (* will remove this *)
+progress; rewrite dom0 in_fset0 in H; elim H.
 trivial.
 proc (LazyInvar IRO.mp{1} BlockIROBitsLazy.mp{2})=> //.
 apply LowerFun_IRO_BlockIROBitsLazy_f.
@@ -385,50 +522,49 @@ local lemma IdealIndifLazy &m :
   Pr[Experiment
      (RaiseBIROBLazy(BlockIROBitsLazy), BlockSim(BlockIROBitsLazy),
       Dist).main() @ &m : res] =
-  Pr[Block.IdealIndif
-     (BlockIROBitsEager, BlockSim, LowerDist(Dist)).main() @ &m : res].
+  Pr[Experiment
+     (RaiseBIROBLazy(BlockIROBitsEager), BlockSim(BlockIROBitsEager),
+      Dist).main() @ &m : res].
 proof.
-byequiv=> //; proc.
-seq 2 2 :
-  (={glob Dist, glob BlockSim} /\ BlockIROBitsLazy.mp{1} = NewFMap.map0 /\
-   BlockIROBitsEager.mp{2} = NewFMap.map0).
-inline *; wp; call (_ : true); auto.
-(* reduction to BlockIROBitsEager *)
+(* reduction to eager *)
 admit.
 qed.
 
 local lemma IdealIndifEager &m :
-  Pr[Block.IdealIndif
-     (BlockIROBitsEager, BlockSim, LowerDist(Dist)).main() @ &m : res] =
-  Pr[Block.IdealIndif
-     (Block.BIRO.IRO, BlockSim, LowerDist(Dist)).main () @ &m : res].
+  Pr[Experiment
+     (RaiseBIROBLazy(BlockIROBitsEager), BlockSim(BlockIROBitsEager),
+      Dist).main() @ &m : res] =
+  Pr[BlockSponge.IdealIndif
+     (BlockSponge.BIRO.IRO, BlockSim, LowerDist(Dist)).main () @ &m : res].
 proof.
 byequiv=> //; proc.
 seq 2 2 :
   (={glob Dist, glob BlockSim} /\ BlockIROBitsEager.mp{1} = NewFMap.map0 /\
-   Block.BIRO.IRO.mp{2} = NewFMap.map0).
+   BlockSponge.BIRO.IRO.mp{2} = NewFMap.map0).
 inline *; wp; call (_ : true); auto.
 call
   (_ :
   ={glob Dist, glob BlockSim} /\
-  BlockIROBitsEager.mp{1} = map0 /\ Block.BIRO.IRO.mp{2} = map0 ==>
+  BlockIROBitsEager.mp{1} = map0 /\ BlockSponge.BIRO.IRO.mp{2} = map0 ==>
   ={res}).
 proc
   (={glob BlockSim} /\
-   EagerInvar Block.BIRO.IRO.mp{2} BlockIROBitsEager.mp{1}) => //.
-smt. (* TODO *)
-proc (EagerInvar Block.BIRO.IRO.mp{2} BlockIROBitsEager.mp{1})=> //;
+   EagerInvar BlockSponge.BIRO.IRO.mp{2} BlockIROBitsEager.mp{1}) => //.
+progress; rewrite dom0 in_fset0 in H; elim H.
+
+proc (EagerInvar BlockSponge.BIRO.IRO.mp{2} BlockIROBitsEager.mp{1})=> //;
   conseq BlockIROBitsEager_BlockIRO_f=> //.
-proc (EagerInvar Block.BIRO.IRO.mp{2} BlockIROBitsEager.mp{1})=> //;
+proc (EagerInvar BlockSponge.BIRO.IRO.mp{2} BlockIROBitsEager.mp{1})=> //;
   conseq BlockIROBitsEager_BlockIRO_f=> //.
-conseq RaiseFun_BlockIROBitsEager_BlockIRO_f=> //.
+exists* n{1}; elim *=> n'.
+conseq RaiseBIROBLazy_BlockIROBitsEager_RaiseFun_Block_IRO_f=> //.
 auto.
 qed.
 
 local lemma IdealIndif &m :
   Pr[IdealIndif(IRO, RaiseSim(BlockSim), Dist).main() @ &m : res] =
-  Pr[Block.IdealIndif
-     (Block.BIRO.IRO, BlockSim, LowerDist(Dist)).main () @ &m : res].
+  Pr[BlockSponge.IdealIndif
+     (BlockSponge.BIRO.IRO, BlockSim, LowerDist(Dist)).main () @ &m : res].
 proof.
 by rewrite (IdealIndifIROLazy &m) (IdealIndifLazy &m) (IdealIndifEager &m).
 qed.
@@ -436,10 +572,10 @@ qed.
 lemma Conclusion' &m :
   `|Pr[RealIndif(Sponge, Perm, Dist).main() @ &m: res] -
     Pr[IdealIndif(IRO, RaiseSim(BlockSim), Dist).main() @ &m : res]| =
-  `|Pr[Block.RealIndif
-       (Block.Sponge, Perm, LowerDist(Dist)).main() @ &m : res] -
-    Pr[Block.IdealIndif
-       (Block.BIRO.IRO, BlockSim, LowerDist(Dist)).main() @ &m : res]|.
+  `|Pr[BlockSponge.RealIndif
+       (BlockSponge.Sponge, Perm, LowerDist(Dist)).main() @ &m : res] -
+    Pr[BlockSponge.IdealIndif
+       (BlockSponge.BIRO.IRO, BlockSim, LowerDist(Dist)).main() @ &m : res]|.
 proof.
 by rewrite (RealIndif &m) (IdealIndif &m).
 qed.
@@ -448,13 +584,13 @@ end section.
 
 (*----------------------------- Conclusion -----------------------------*)
 
-lemma Conclusion (BlockSim <: Block.SIMULATOR{IRO, Block.BIRO.IRO})
-                 (Dist <: DISTINGUISHER{Perm, BlockSim, IRO, Block.BIRO.IRO})
+lemma Conclusion (BlockSim <: BlockSponge.SIMULATOR{IRO, BlockSponge.BIRO.IRO})
+                 (Dist <: DISTINGUISHER{Perm, BlockSim, IRO, BlockSponge.BIRO.IRO})
                  &m :
   `|Pr[RealIndif(Sponge, Perm, Dist).main() @ &m: res] -
     Pr[IdealIndif(IRO, RaiseSim(BlockSim), Dist).main() @ &m : res]| =
-  `|Pr[Block.RealIndif
-       (Block.Sponge, Perm, LowerDist(Dist)).main() @ &m : res] -
-    Pr[Block.IdealIndif
-       (Block.BIRO.IRO, BlockSim, LowerDist(Dist)).main() @ &m : res]|.
+  `|Pr[BlockSponge.RealIndif
+       (BlockSponge.Sponge, Perm, LowerDist(Dist)).main() @ &m : res] -
+    Pr[BlockSponge.IdealIndif
+       (BlockSponge.BIRO.IRO, BlockSim, LowerDist(Dist)).main() @ &m : res]|.
 proof. by apply/(Conclusion' BlockSim Dist &m). qed.
